Communication_Topology_Soundness.thy
@@ -9,17 +9,18 @@ begin
 theorem topology_pair_sound : "
   \<lbrakk>
     (x, t) \<Turnstile>\<^sub>t e; 
-    [[] \<mapsto> <<e, empty, []>>] \<rightarrow>* \<E>';
-    \<E>' \<pi> = Some (<<LET x' = CHAN \<lparr>\<rparr> in e', \<rho>', \<kappa>'>>)
+    [[] \<mapsto> <<e, empty, []>>] \<rightarrow>* \<E>'
   \<rbrakk> \<Longrightarrow>
-  \<langle>\<langle>\<E>' ; Ch \<pi> x\<rangle>\<rangle> \<preceq> t
+  \<langle>\<langle>\<E>' ; x\<rangle>\<rangle> \<preceq> t
 "
 sorry
 
 lemma topology_sound': "
   (x, \<A> x) \<Turnstile>\<^sub>t e \<Longrightarrow> [[] \<mapsto> <<e,Map.empty,[]>>] \<rightarrow>* \<E>' \<Longrightarrow> (\<langle>\<langle>\<E>'\<rangle>\<rangle>) x \<preceq> \<A> x
 "
-sorry
+ apply (drule topology_pair_sound, simp)
+ apply (unfold state_pool_to_topo_env_def, auto)
+done
 
 theorem topology_sound : "
   \<lbrakk>
@@ -28,11 +29,10 @@ theorem topology_sound : "
   \<rbrakk> \<Longrightarrow>
   \<langle>\<langle>\<E>'\<rangle>\<rangle> \<sqsubseteq>\<^sub>t \<A>
 "
- apply (unfold communication_topology_def)
+ apply (unfold topo_accept_def)
  apply (unfold topo_env_precision_def)
  apply (intro allI, drule spec)
  apply (erule topology_sound', auto)
 done
- 
 
 end
